minuska/lib/micoqprint.ml
@@ -23,7 +23,6 @@ Instance LangDefaults : Defaults := {|
     default_context_template := myContext ;
 
     default_isValue := isValue ;
-    default_isNonValue := isNonValue ;
 |}.
 |delimiter}
 
@@ -168,7 +167,7 @@ let rec print_exprterm
     myiter (fun x -> print_exprterm iface my_builtins_map my_query_map name_of_builtins oux x; ()) (fun () -> fprintf oux "; "; ()) ps;
     fprintf oux "])"
 
-let print_cond_w_hole
+let rec print_cond_w_hole
   (iface : 'a Dsm.builtinInterface)
   (my_builtins_map : builtins_map_t)
   (my_query_map : query_map_t)
@@ -178,10 +177,32 @@ let print_cond_w_hole
   (hole : string option)
   : unit =
   match c with
-  | `Cond (`Id s, es) ->
-      fprintf oux "(mkSideCondition2 _ %s [" (snd (translate_name my_builtins_map my_query_map s));
+  | `CondAtomic (`Id s, es) ->
+      fprintf oux "(sc_atom %s [" (snd (translate_name my_builtins_map my_query_map s));
       myiter (fun x -> print_expr_w_hole iface my_builtins_map my_query_map name_of_builtins oux x hole; ()) (fun () -> fprintf oux "; "; ()) es;
       fprintf oux "])"
+  | `CondAnd (c1, c2) -> (
+    fprintf oux "(sc_and ";
+    print_cond_w_hole iface my_builtins_map my_query_map name_of_builtins oux c1 hole;
+    print_cond_w_hole iface my_builtins_map my_query_map name_of_builtins oux c2 hole;
+    fprintf oux ")";
+    ()
+  )
+  | `CondOr (c1, c2) -> (
+      fprintf oux "(sc_or ";
+      print_cond_w_hole iface my_builtins_map my_query_map name_of_builtins oux c1 hole;
+      print_cond_w_hole iface my_builtins_map my_query_map name_of_builtins oux c2 hole;
+      fprintf oux ")";
+      ()
+  )
+  | `CondTrue -> (
+    fprintf oux "sc_true";
+    ()
+  )
+  | `CondFalse -> (
+    fprintf oux "sc_false";
+    ()
+  )
 
 
 
@@ -205,9 +226,10 @@ let print_rule
     fprintf oux " ";
     print_exprterm iface my_builtins_map my_query_map name_of_builtins oux (r.rhs);
     fprintf oux " ";
-    fprintf oux "[";
-    myiter (fun x -> print_cond_w_hole iface my_builtins_map my_query_map name_of_builtins oux x None; ()) (fun () -> fprintf oux "; "; ()) (r.cond);
-    fprintf oux "]";
+    print_cond_w_hole iface my_builtins_map my_query_map name_of_builtins oux r.cond None;
+    (* fprintf oux "["; *)
+    (* myiter (fun x -> print_cond_w_hole iface my_builtins_map my_query_map name_of_builtins oux x None; ()) (fun () -> fprintf oux "; "; ()) (r.cond); *)
+    (* fprintf oux "]"; *)
     fprintf oux ")\n";
     ()
 
@@ -223,7 +245,7 @@ let print_strict oux str =
   fprintf oux "(decl_strict (mkStrictnessDeclaration _ \"%s\" %d " (match str.symbol with `Id s -> s) (str.arity) ;
   fprintf oux "[";
   myiter (fun x -> fprintf oux "%d" x; ()) (fun () -> fprintf oux "; "; ()) (str.strict_places);
-  fprintf oux "] isValue isNonValue myContext";
+  fprintf oux "] isValue _ myContext";
   fprintf oux "))\n";
   ()
 
@@ -258,11 +280,7 @@ let print_definition
     print_cond_w_hole iface my_builtins_map my_query_map name_of_builtins oux (snd (def.Syntax.value)) (Some (match (fst (def.Syntax.value)) with `Var s -> s));
     fprintf oux ".\n";
     
-    fprintf oux "Definition isNonValue (";
-    fprintf oux "%s" (match (fst (def.Syntax.nonvalue)) with `Var s -> s);
-    fprintf oux " : Expression2) := ";
-    print_cond_w_hole iface my_builtins_map my_query_map (name_of_builtins : string) oux (snd (def.Syntax.nonvalue)) (Some (match (fst (def.Syntax.nonvalue)) with `Var s -> s));
-    fprintf oux ".\n";
+    fprintf oux "#[export] Instance isValue_nsc (X : Expression2) : NegableSideCondition (isValue X) := ltac:(intros; unfold isValue in *; apply _).\n";
     
     fprintf oux "%s\n" output_part_2;
     List.iter ~f:(fun fr -> print_frame oux fr) (def.frames);
