minuska/lib/parser.mly
@@ -2,7 +2,6 @@
 %token <string> ID
 %token <string> VAR
 %token KEYWORD_VALUE
-%token KEYWORD_NONVALUE
 %token KEYWORD_STRICTNESS
 %token KEYWORD_BUILTIN_INT
 %token KEYWORD_BUILTIN_STRING
@@ -12,6 +11,10 @@
 %token KEYWORD_IN
 %token KEYWORD_WHERE
 %token KEYWORD_CONTEXT
+%token KEYWORD_TRUE
+%token KEYWORD_FALSE
+%token KEYWORD_AND
+%token KEYWORD_OR
 %token BRACKET_ROUND_LEFT
 %token BRACKET_ROUND_RIGHT
 %token BRACKET_SQUARE_LEFT
@@ -116,11 +119,29 @@ expr:
   ;
 
 condition:
+  | KEYWORD_TRUE
+    { `CondTrue }
+  | KEYWORD_FALSE
+    { `CondFalse }
   | p = ID
     BRACKET_ROUND_LEFT
     es = separated_list(COMMA, expr)
     BRACKET_ROUND_RIGHT
-    { `Cond ((`Id p), es) }
+    { `CondAtomic ((`Id p), es) }
+  | KEYWORD_OR
+    BRACKET_ROUND_LEFT
+    c1 = condition
+    COMMA
+    c2 = condition
+    BRACKET_ROUND_RIGHT
+    { `CondOr (c1, c2) }
+  | KEYWORD_AND
+    BRACKET_ROUND_LEFT
+    c1 = condition
+    COMMA
+    c2 = condition
+    BRACKET_ROUND_RIGHT
+    { `CondAnd (c1, c2) }
   ;
 
 exprterm:
@@ -139,22 +160,9 @@ valuedecl:
     x = VAR 
     BRACKET_ROUND_RIGHT
     COLON 
-    BRACKET_ROUND_LEFT
+    // BRACKET_ROUND_LEFT
     c = condition
-    BRACKET_ROUND_RIGHT
-    SEMICOLON
-    { (x,c) }
-  ;
-
-nonvaluedecl:
-  | KEYWORD_NONVALUE
-    BRACKET_ROUND_LEFT
-    x = VAR 
-    BRACKET_ROUND_RIGHT
-    COLON 
-    BRACKET_ROUND_LEFT
-    c = condition
-    BRACKET_ROUND_RIGHT
+    // BRACKET_ROUND_RIGHT
     SEMICOLON
     { (x,c) }
   ;
@@ -196,21 +204,21 @@ rule:
     ARROW
     r = exprterm
     KEYWORD_WHERE
-    BRACKET_SQUARE_LEFT
-    cs = separated_list(COMMA, condition);
-    BRACKET_SQUARE_RIGHT
+    // BRACKET_SQUARE_LEFT
+    c = condition
+    // cs = separated_list(COMMA, condition);
+    // BRACKET_SQUARE_RIGHT
     SEMICOLON
-    { {frame = a; name = n; lhs = l; rhs = r; cond = cs }  }
+    { {frame = a; name = n; lhs = l; rhs = r; cond = c }  }
   ;
 
 definition:
   | fs = framesdecl
     v = valuedecl
-    nv = nonvaluedecl
     c = contextdecl
     sall = strictnessall
     rs = list(rule)
-    { { context = c; value = (`Var (fst v), (snd v)); nonvalue = (`Var (fst nv), (snd nv)); frames = fs; strictness = sall; rules = rs } }
+    { { context = c; value = (`Var (fst v), (snd v)); frames = fs; strictness = sall; rules = rs } }
   ;
 
 option_definition:
