coq-minuska/theories/prelude.v
@@ -1087,6 +1087,343 @@ Proof.
     }
 Qed.
 
+Lemma fmap_Some_T_1 (A B : Type) (f : A → B) (mx : option A) (y : B):
+  f <$> mx = Some y ->
+  {x : A & mx = Some x ∧ y = f x }
+.
+Proof.
+    intros H.
+    destruct mx; simpl in *.
+    {
+        inversion H; subst; clear H.
+        exists a.
+        split;reflexivity.
+    }
+    {
+        inversion H.
+    }
+Qed.
+
+
+Lemma sum_list_with_pairwise
+    {T1 T2 : Type}
+    (f1 : T1 -> nat)
+    (f2 : T2 -> nat)
+    (l1 : list T1)
+    (l2 : list T2)
+    :
+    length l1 = length l2 ->
+    (forall i x1 x2, l1!!i = Some x1 -> l2!!i = Some x2 -> f1 x1 >= f2 x2) ->
+    sum_list_with f1 l1 >= sum_list_with f2 l2
+.
+Proof.
+    revert l2.
+    induction l1; intros l2 Hlen H; destruct l2; simpl in *; try ltac1:(lia).
+    {
+        specialize (IHl1 l2 ltac:(lia)).
+        assert (H' := H 0 a t eq_refl eq_refl).
+        ltac1:(cut (sum_list_with f1 l1 ≥ sum_list_with f2 l2)).
+        {
+            intros HH. ltac1:(lia).
+        }
+        apply IHl1. intros.
+        specialize (H (S i) x1 x2 H0 H1).
+        apply H.
+    }
+Qed.
+
+Lemma sum_list_with_eq_pairwise
+    {T1 T2 : Type}
+    (f1 : T1 -> nat)
+    (f2 : T2 -> nat)
+    (l1 : list T1)
+    (l2 : list T2)
+    :
+    length l1 = length l2 ->
+    (forall i x1 x2, l1!!i = Some x1 -> l2!!i = Some x2 -> f1 x1 = f2 x2) ->
+    sum_list_with f1 l1 = sum_list_with f2 l2
+.
+Proof.
+    revert l2.
+    induction l1; intros l2 Hlen H; destruct l2; simpl in *; try ltac1:(lia).
+    {
+        specialize (IHl1 l2 ltac:(lia)).
+        assert (H' := H 0 a t eq_refl eq_refl).
+        ltac1:(cut (sum_list_with f1 l1 = sum_list_with f2 l2)).
+        {
+            intros HH. ltac1:(lia).
+        }
+        apply IHl1. intros.
+        specialize (H (S i) x1 x2 H0 H1).
+        apply H.
+    }
+Qed.
+
+Lemma sum_list_with_eq_plus_pairwise
+    {T1 T2 : Type}
+    (f1 : T1 -> nat)
+    (f2 : T2 -> nat)
+    (g : T2 -> nat)
+    (l1 : list T1)
+    (l2 : list T2)
+    :
+    length l1 = length l2 ->
+    (forall i x1 x2, l1!!i = Some x1 -> l2!!i = Some x2 -> f1 x1 = f2 x2 + g x2) ->
+    sum_list_with f1 l1 = sum_list_with f2 l2 + sum_list_with g l2
+.
+Proof.
+    revert l2.
+    induction l1; intros l2 Hlen H; destruct l2; simpl in *; try ltac1:(lia).
+    {
+        specialize (IHl1 l2 ltac:(lia)).
+        assert (H' := H 0 a t eq_refl eq_refl).
+        ltac1:(cut (sum_list_with f1 l1 = sum_list_with f2 l2 + sum_list_with g l2)).
+        {
+            intros HH. ltac1:(lia).
+        }
+        apply IHl1. intros.
+        specialize (H (S i) x1 x2 H0 H1).
+        apply H.
+    }
+Qed.
+
+
+
+
+Lemma list_filter_Forall_all
+    {T : Type}
+    (P : T -> Prop)
+    {_dP : forall x, Decision (P x)}
+    (l : list T)
+    :
+    Forall P l ->
+    filter P l = l
+.
+Proof.
+    induction l; simpl; intros H.
+    {
+        reflexivity.
+    }
+    {
+        apply Forall_cons in H.
+        destruct H as [H1 H2].
+        specialize (IHl H2). clear H2.
+        rewrite filter_cons.
+        destruct (decide (P a)).
+        {
+            rewrite IHl. reflexivity.
+        }
+        ltac1:(contradiction).
+    }
+Qed.
+
+
+Lemma count_one_split
+    {T : Type}
+    (P : T -> Prop)
+    (_dP : forall x, Decision (P x))
+    (l : list T)
+    :
+    length (filter P l) = 1 ->
+    exists (la : list T) (b : T) (lc : list T),
+    l = la ++ b::lc
+    /\ P b
+    /\ Forall (fun x => not (P x)) la
+    /\ Forall (fun x => not (P x)) lc
+.
+Proof.
+    remember (list_find P l) as lf.
+    destruct lf.
+    {
+        symmetry in Heqlf.
+        destruct p.
+        apply list_find_Some in Heqlf.
+        intros HH.
+        destruct Heqlf as [H1 [H2 H3]].
+        apply take_drop_middle in H1.
+        exists (take n l).
+        exists t.
+        exists (drop (S n) l).
+        split.
+        {
+            symmetry. exact H1.
+        }
+        split>[exact H2|].
+        split.
+        {
+            rewrite Forall_forall.
+            intros x Hx.
+            rewrite elem_of_list_lookup in Hx.
+            destruct Hx as [i Hi].
+            rewrite lookup_take_Some in Hi.
+            destruct Hi as [Hi H'i].
+            eapply H3.
+            { apply Hi. }
+            { apply H'i. }
+        }
+        {
+            rewrite Forall_forall.
+            intros x Hx HContra.
+            rewrite elem_of_list_lookup in Hx.
+            destruct Hx as [i Hi].
+            apply take_drop_middle in Hi.
+            rewrite <- Hi in H1.
+            rewrite <- H1 in HH.
+            clear H1 Hi.
+            rewrite filter_app in HH.
+            rewrite filter_cons in HH.
+            destruct (decide (P t))>[|ltac1:(contradiction)].
+            rewrite filter_app in HH.
+            rewrite filter_cons in HH.
+            destruct (decide (P x))>[|ltac1:(contradiction)].
+            rewrite length_app in HH. simpl in HH.
+            rewrite length_app in HH. simpl in HH.
+            ltac1:(lia).
+        }
+    }
+    {
+        symmetry in Heqlf.
+        apply list_find_None in Heqlf.
+        intros Hlength.
+        apply length_filter_l_1_impl_h_in_l' in Hlength.
+        destruct Hlength as [h [H1h H2h]].
+        rewrite Forall_forall in Heqlf.
+        ltac1:(exfalso).
+        ltac1:(naive_solver).
+    }
+Qed.
+
+
+Lemma sum_list_with_perm
+    {T : Type}
+    (f : T -> nat)
+    (l1 l2 : list T)
+    :
+    l1 ≡ₚ l2 ->
+    sum_list_with f l1 = sum_list_with f l2
+.
+Proof.
+    intros H.
+    induction H.
+    {
+        reflexivity.
+    }
+    {
+        simpl. rewrite IHPermutation. reflexivity.
+    }
+    {
+        simpl. ltac1:(lia).
+    }
+    {
+        ltac1:(congruence).
+    }
+Qed.
+
+Lemma flat_map_lookup_Some
+    {A B : Type}
+    (f : A -> list B)
+    (l : list A)
+    (i : nat)
+    (y : B)
+    :
+    (flat_map f l) !! i = Some y ->
+    { j : nat & { x : A & { k : nat & l !! j = Some x /\ (f x) !! k = Some y } } }
+.
+Proof.
+    revert i.
+    induction l; simpl; intros i HH.
+    {
+        rewrite lookup_nil in HH.
+        inversion HH.
+    }
+    {
+        destruct (decide (i < length (f a))) as [Hlt|Hgeq].
+        {
+            rewrite lookup_app_l in HH>[|exact Hlt].
+            exists 0.
+            exists a.
+            exists i.
+            simpl.
+            split>[reflexivity|].
+            exact HH.            
+        }
+        {
+            rewrite lookup_app_r in HH.
+            specialize (IHl _ HH).
+            destruct IHl as [j [x [k [H1 H2]]]].
+            exists (S j).
+            exists x.
+            exists k.
+            simpl.
+            split>[apply H1|].
+            exact H2.
+            ltac1:(lia).
+        }
+    }
+Qed.
+
+
 Inductive MyUnit := mytt.
 
+
+Definition slice {A : Type} {_eqA : EqDecision A} (from : nat) (to : nat) (l : list A) :=
+    take (to - from) (drop from l)
+.
+
+Ltac2 simplify_fmap_eq () :=
+    repeat (
+        match! goal with
+        | [h: ([] = (_ <$> _)) |- _] =>
+            symmetry in $h
+        | [h: (_::_ = (_ <$> _)) |- _] =>
+            symmetry in $h
+        | [h: ((?f <$> ?l) = []) |- _] =>
+            apply fmap_nil_inv in $h; subst
+        | [h: ((?f <$> ?l) = (?x::?xs)) |- _] =>
+            apply fmap_cons_inv in $h;
+            Std.destruct
+                false
+                [{
+                    Std.indcl_arg := Std.ElimOnIdent(h);
+                    Std.indcl_eqn := None;
+                    Std.indcl_as := Some(Std.IntroAndPattern(
+                        [
+                            Std.IntroNaming(Std.IntroAnonymous);
+                            Std.IntroAction(
+                                Std.IntroOrAndPattern(Std.IntroAndPattern([
+                                    Std.IntroNaming(Std.IntroAnonymous);
+                                    Std.IntroNaming(Std.IntroAnonymous)
+                                ]))
+                            )
+                        ]
+                        )) ;
+                    Std.indcl_in := None;
+                }]
+                None;
+            ltac1:(destruct_and?);
+            subst; simpl in *;
+            ()
+        end
+    )
+.
+
+Search drop S.
+Ltac2 simplify_take_drop () :=
+    repeat (
+        match! goal with
+        | [h: context c [take 0 _] |- _] =>
+            rewrite take_0 in $h
+        | [h: context c [drop 0 _] |- _] =>
+            rewrite drop_0 in $h
+        | [h: context c [take (S _) (_::_)] |- _] =>
+            rewrite firstn_cons in $h; simpl in *
+        | [h: context c [take (S _) ?l] |- _] =>
+            destruct $l; simpl in *
+        | [h: context c [drop (S _) (_::_)] |- _] =>
+            rewrite skipn_cons in $h; simpl in *
+        | [h: context c [drop (S _) ?l] |- _] =>
+            destruct $l; simpl in *
+        end
+    )
+.
 
