coq-minuska/theories/basic_properties.v
@@ -387,9 +387,9 @@ End custom_induction_principle_2.
 Existing Instance Expression2_eqdec.
 
 #[export]
-Instance SideCondition2_eqdec
+Instance SideCondition_eqdec
     {Σ : StaticModel}
-    : EqDecision (SideCondition2)
+    : EqDecision (SideCondition)
 .
 Proof. ltac1:(solve_decision). Defined.
 
@@ -467,6 +467,21 @@ match e with
 end
 .
 
+Fixpoint SideCondition_subst
+    {Σ : StaticModel}
+    (c : SideCondition)
+    (x : variable)
+    (e' : Expression2)
+    : SideCondition
+:=
+    match c with
+    | sc_true => sc_true
+    | sc_false => sc_false
+    | sc_atom p es => sc_atom p ((fun e1 => Expression2_subst e1 x e') <$> es)
+    | sc_and l r => sc_and (SideCondition_subst l x e') (SideCondition_subst r x e')
+    | sc_or l r => sc_or (SideCondition_subst l x e') (SideCondition_subst r x e')
+    end
+.
 
 Fixpoint vars_of_to_l2r
     {Σ : StaticModel}
@@ -812,3 +827,15 @@ Proof.
         }
     }
 Qed.
+
+
+Lemma TermOver_size_not_zero
+    {Σ : StaticModel}
+    {A : Type}
+    (t : TermOver A)
+    : TermOver_size t <> 0
+.
+Proof.
+    destruct t; simpl; ltac1:(lia).
+Qed.
+
