coq-minuska/theories/minusl_semantics.v
@@ -33,15 +33,15 @@ Section MinusL_sem.
             (lc : TermOver BuiltinOrVar) (ld : TermOver BuiltinOrVar)
             (a : Act)
             (rc : TermOver Expression2) (rd : TermOver Expression2)
-            (scs : list SideCondition2),
-            (mld_rewrite Act lc ld a rc rd scs) ∈ (mlld_decls Act D) ->
+            (c : SideCondition),
+            (mld_rewrite Act lc ld a rc rd c) ∈ (mlld_decls Act D) ->
         forall (ctrl1 state1 ctrl2 state2 : TermOver builtin_value) (nv : NondetValue)
             (ρ : Valuation2),
             satisfies ρ ctrl1 lc ->
             satisfies ρ state1 ld ->
             satisfies ρ (program, (nv,ctrl2)) rc ->
             satisfies ρ (program, (nv,state2)) rd ->
-            satisfies ρ (program, nv) scs ->
+            satisfies ρ (program, nv) c ->
         MinusL_rewrites D program ctrl1 state1 [a] ctrl2 state2
 
     | mlr_trans :
@@ -54,19 +54,19 @@ Section MinusL_sem.
 
     | mlr_context :
         forall
-            (c : TermOver BuiltinOrVar)
+            (ctx : TermOver BuiltinOrVar)
             (h : variable)
-            (scs : list SideCondition2),
-            (mld_context Act c h scs) ∈ (mlld_decls Act D) ->
+            (c : SideCondition),
+            (mld_context Act ctx h c) ∈ (mlld_decls Act D) ->
         forall (ctrl1 state1 ctrl2 state2 r v : TermOver builtin_value)
             (w : list Act)
             (ρ1 : Valuation2)
             (ρ2 : Valuation2)
             (nv : NondetValue),
-            (∀ x, x ∈ vars_of_to_l2r c -> x <> h -> ρ1 !! x = ρ2 !! x) ->
-            satisfies (<[h := r]>ρ1) ctrl1 c ->
-            satisfies ρ1 (program, nv) scs ->
-            satisfies (<[h := v]>ρ2) ctrl2 c ->
+            (∀ x, x ∈ vars_of ctx -> x <> h -> ρ1 !! x = ρ2 !! x) ->
+            satisfies (<[h := r]>ρ1) ctrl1 ctx ->
+            satisfies ρ1 (program, nv) c ->
+            satisfies (<[h := v]>ρ2) ctrl2 ctx ->
             satisfies ρ2 (program, nv) (MinusL_isValue Act D (e_ground v)) ->
             MinusL_rewrites D program r state1 w v state2 ->
             MinusL_rewrites D program ctrl1 state1 w ctrl2 state2
