languages/imp/imp.m
@@ -1,18 +1,8 @@
 @frames: [
   simple(X): c[builtin.cseq [X,REST], STATE]
 ];
-@value(X): (is_true (bool.or(
-   z.is(X),                            bool.or(
-   bool.is(X),                         bool.or(
-    term.same_symbol(X, [unitValue[]]), 
-   string.is(X)
-))))) ;
-@nonvalue(X): (is_true (bool.neg(bool.or(
-   z.is(X),                            bool.or(
-   bool.is(X),                         bool.or(
-   term.same_symbol(X, [unitValue[]]), 
-   string.is(X)
-)))))) ;
+@value(X): @or(z.is(X), @or(string.is(X), @or(bool.is(X), term.same_symbol(X, [unitValue[]]))));
+
 @context(HOLE): c[HOLE, STATE];
 @strictness: [
   plus of_arity 2 in [0,1],
@@ -27,27 +17,27 @@
 ];
 
 
-@rule [init]: builtin.init[] => c[builtin.cseq[program.ast(), builtin.empty_cseq[]], map.empty()] where [];
+@rule [init]: builtin.init[] => c[builtin.cseq[program.ast(), builtin.empty_cseq[]], map.empty()] where @true ;
 
-@rule/simple [aexpr.plus]: plus[X,Y] => z.plus(X, Y) where [is_true(z.is(X)), is_true(z.is(Y))] ;
-@rule/simple [aexpr.minus]: minus[X,Y] => z.minus(X, Y) where [is_true(z.is(X)), is_true(z.is(Y))] ;
+@rule/simple [aexpr.plus]: plus[X,Y] => z.plus(X, Y) where @and(z.is(X), z.is(Y)) ;
+@rule/simple [aexpr.minus]: minus[X,Y] => z.minus(X, Y) where @and(z.is(X), z.is(Y)) ;
 
 @rule [var.assign]: c[builtin.cseq[assign[X,V],REST], STATE]
   => c[builtin.cseq[unitValue[], REST], map.update(STATE, X, V)]
-   where [is_true(term.same_symbol(X, [var[]])), is_true(bool.or(z.is(V), string.is(V)))] ;
+   where @and(term.same_symbol(X, [var[]]), @or(z.is(V), string.is(V))) ;
 
-@rule [var.lookup]: c[builtin.cseq[X, REST], STATE] => c[builtin.cseq[map.lookup(STATE, X), REST], STATE] where [is_true(term.same_symbol(X, [var[]]))] ;
+@rule [var.lookup]: c[builtin.cseq[X, REST], STATE] => c[builtin.cseq[map.lookup(STATE, X), REST], STATE] where term.same_symbol(X, [var[]]) ;
 
-@rule/simple [stmt.seq]: seq[unitValue[], X] => X where [] ;
+@rule/simple [stmt.seq]: seq[unitValue[], X] => X where @true ;
 
-@rule/simple [bexpr.eq]: eq[X, Y] => z.eq(X, Y) where [is_true(z.is(X)), is_true(z.is(Y))] ;
-@rule/simple [bexpr.le]: le[X, Y] => z.le(X, Y) where [is_true(z.is(X)), is_true(z.is(Y))] ;
-@rule/simple [bexpr.lt]: lt[X, Y] => z.lt(X, Y) where [is_true(z.is(X)), is_true(z.is(Y))] ;
-@rule/simple [bexpr.neg]: not[X] => bool.neg(X) where [is_true(bool.is(X))] ;
+@rule/simple [bexpr.eq]: eq[X, Y] => z.eq(X, Y) where @and(z.is(X), z.is(Y)) ;
+@rule/simple [bexpr.le]: le[X, Y] => z.le(X, Y) where @and(z.is(X), z.is(Y)) ;
+@rule/simple [bexpr.lt]: lt[X, Y] => z.lt(X, Y) where @and(z.is(X), z.is(Y)) ;
+@rule/simple [bexpr.neg]: not[X] => bool.neg(X) where bool.is(X) ;
 
-@rule/simple [stmt.ite.true]: ite[B, X, Y] => X where [is_true(bool.is(B)), is_true(bool.eq(B, bool.true()))] ;
-@rule/simple [stmt.ite.false]: ite[B, X, Y] => Y where [is_true(bool.is(B)), is_true(bool.eq(B, bool.false()))] ;
+@rule/simple [stmt.ite.true]:  ite[B, X, Y] => X where @and(bool.is(B), bool.is_true(B)) ;
+@rule/simple [stmt.ite.false]: ite[B, X, Y] => Y where @and(bool.is(B), bool.is_false(B)) ;
 
-@rule/simple [while.unfold]: while[B, S] => ite[B, seq[S, while[B, S]], unitValue[]] where [] ;
+@rule/simple [while.unfold]: while[B, S] => ite[B, seq[S, while[B, S]], unitValue[]] where @true ;
 
 
